refactor: Introduce the [MayProvide] typeclass, stop using [state_t]
This patch introduces at least two significant refactoring. They are
committed together because they are deeply tied and have been
implemented at once (changes induce by one impacting the other).

With respect to the verification formalism:

  - When reasoning on an impure computation trustworthiness, the
    interface of the computation does not have to be the same as the
    specification.  It is just require that there is an instance of
    the [MayProvide] typeclass to select primitives used by the
    impure computation that are concerned by the specification

  - The same approach has also been implemented for semantics
    compliance.

  - The [specsplus] operator has been changed, and allows for more
    easily composed specification.  This remains to be formally
    proven, but this new operator is symmetric (c <.> c' ~~ c' <.> c)
    and associative (c <.> (c' <.> c'') ~~ (c <.> c') <.> c'').

    A major advantage of this approach is that it becomes possible to
    compose specification of the same interface together. A drawback,
    however, is that composing the same interface twice does not make
    sense anymore (that is, i <+> i is morally equivalent to i). Note
    that, from the perspective of the [Provide] typeclass, this was
    already the case.

With respect to the component formalism:

  - The component becomes stateless, and therefore a mere proxy from
    the interface it exposes to the interface it used.  A component
    can rely on an external state thanks to the [STORE] interface.

  - The different related definitions have been updated to reflect
    this change.

core/examples/airlock.v
@@ -37,18 +37,18 @@ Inductive DOORS : interface :=
 
 Generalizable All Variables.
 
-Definition is_open `{ix :| DOORS} (d : door) : impure ix bool :=
+Definition is_open `{Provide ix DOORS} (d : door) : impure ix bool :=
   request (IsOpen d).
 
-Definition toggle `{ix :| DOORS} (d : door) : impure ix unit :=
+Definition toggle `{Provide ix DOORS} (d : door) : impure ix unit :=
   request (Toggle d).
 
-Definition open_door `{ix :| DOORS} (d : door) : impure ix unit :=
+Definition open_door `{Provide ix DOORS} (d : door) : impure ix unit :=
   do var open <- is_open d in
      when (negb open) (toggle d)
   end.
 
-Definition close_door `{ix :| DOORS} (d : door) : impure ix unit :=
+Definition close_door `{Provide ix DOORS} (d : door) : impure ix unit :=
   do var open <- is_open d in
      when open (toggle d)
    end.
@@ -59,10 +59,10 @@ Inductive CONTROLLER : interface :=
 | Tick : CONTROLLER unit
 | RequestOpen (d : door) : CONTROLLER unit.
 
-Definition tick `{ix :| CONTROLLER} : impure ix unit :=
+Definition tick `{Provide ix CONTROLLER} : impure ix unit :=
   request Tick.
 
-Definition request_open `{ix :| CONTROLLER} (d : door) : impure ix unit :=
+Definition request_open `{Provide ix CONTROLLER} (d : door) : impure ix unit :=
   request (RequestOpen d).
 
 Definition co (d : door) : door :=
@@ -71,22 +71,20 @@ Definition co (d : door) : door :=
   | right => left
   end.
 
-From Prelude Require Import State.
-
-Definition controller : component CONTROLLER DOORS nat :=
+Definition controller `{Provide ix DOORS, Provide ix (STORE nat)} : component CONTROLLER ix :=
   fun _ op =>
     match op with
     | Tick =>
       do var cpt <- get in
          when (15 <? cpt) do
-           lift (close_door left);
-           lift (close_door right);
+           close_door left;
+           close_door right;
            put 0
          end
       end
     | RequestOpen d => do
-        lift (close_door (co d));
-        lift (open_door d);
+        close_door (co d);
+        open_door d;
         put 0
       end
     end.
@@ -132,7 +130,7 @@ Qed.
     trick to prevent [cbn] to unfold impure computations covered by intermediary
     theorems. *)
 
-#[local] Arguments tog : simpl never.
+#[local] Opaque tog.
 
 Definition step (ω : Ω) (a : Type) (e : DOORS a) (x : a) :=
   match e with
@@ -178,7 +176,7 @@ Definition doors_specs : specs DOORS Ω := Build_specs _ _ step req prom.
 
 (** Closing a door [d] in any system [ω] is always a trustworthy operation. *)
 
-Lemma close_door_trustworthy (ω : Ω) (d : door)
+Lemma close_door_trustworthy `{Provide ix DOORS} (ω : Ω) (d : door)
   : trustworthy_impure doors_specs ω (close_door d).
 
 Proof.
@@ -191,38 +189,35 @@ Proof.
      Yet, thanks to our call to [IsOpen d], we can predict that
 
        [sel d ω = true] *)
-  inversion Hpost; ssubst.
-  now rewrite H1.
+  inversion prom0; ssubst.
+  now rewrite H3.
 Qed.
 
-Lemma open_door_trustworthy (ω : Ω) (d : door) (safe : sel (co d) ω = false)
-  : trustworthy_impure doors_specs ω (open_door d).
+Lemma open_door_trustworthy `{Provide ix DOORS} (ω : Ω)
+    (d : door) (safe : sel (co d) ω = false)
+  : trustworthy_impure doors_specs ω (open_door (ix := ix) d).
 
 Proof.
   prove_impure; cbn; repeat constructor; subst.
-  inversion Hpost; ssubst.
+  inversion prom0; ssubst.
   now rewrite safe.
 Qed.
 
-Lemma close_door_run (ω : Ω) (d : door) (ω' : Ω) (x : unit)
-  (run : trustworthy_run doors_specs (close_door d) ω ω' x)
+Lemma close_door_run `{Provide ix DOORS} (ω : Ω) (d : door) (ω' : Ω) (x : unit)
+  (run : trustworthy_run doors_specs (close_door (ix := ix) d) ω ω' x)
   : sel d ω' = false.
+
 Proof.
-  inversion run; ssubst; clear run req0; cbn in *.
-  inversion prom0; ssubst; clear prom0.
-  case_eq (sel d ω); intros equ; rewrite equ in rec;
-    inversion rec; ssubst; cbn in *; try clear req.
-  + inversion rec0; ssubst; clear rec0.
-    rewrite tog_equ_1.
-    rewrite equ.
-    reflexivity.
-  + inversion rec; ssubst; clear rec.
-    exact equ.
+  unroll_impure_run run; cbn in *.
+  + rewrite tog_equ_1.
+    inversion prom0; ssubst.
+    now rewrite H3.
+  + now inversion prom0; ssubst.
 Qed.
 
-#[local] Arguments close_door : simpl never.
-#[local] Arguments open_door : simpl never.
-#[local] Arguments Nat.ltb : simpl never.
+#[local] Opaque close_door.
+#[local] Opaque open_door.
+#[local] Opaque Nat.ltb.
 
 Fact one_door_safe_all_doors_safe (ω : Ω) (d : door)
     (safe : sel d ω = false \/ sel (co d) ω = false)
@@ -242,11 +237,12 @@ Qed.
     the left door is closed, then after any trustworthy run of a computation
     [p], this fact remains true. *)
 
-Lemma trustworthy_run_inv {a} (p : impure DOORS a)
+Lemma trustworthy_run_inv `{Provide ix DOORS} {a} (p : impure ix a)
   (ω : Ω) (safe : sel left ω = false \/ sel right ω = false)
   (x : a) (ω' : Ω) (run : trustworthy_run doors_specs p ω ω' x)
   : sel left ω' = false \/ sel right ω' = false.
 
+#[local] Opaque sel.
 
 (** We reason by induction on the impure computation [p]:
 
@@ -284,42 +280,52 @@ Proof.
   induction p; intros ω run safe.
   + now unroll_impure_run run.
   + unroll_impure_run run.
-    eapply H; eauto.
-    destruct e as [d|d]; cbn -[sel] in *; auto.
-    (* We try to toggle a door [d]. *)
-    apply one_door_safe_all_doors_safe with (d := d).
-    apply one_door_safe_all_doors_safe with (d' := d) in safe.
-    inversion req0; ssubst.
-    destruct safe as [safe | safe].
+    destruct (unlift_eff e) as [ e' |].
+    ++ eapply H1; eauto.
+       destruct e' as [d|d]; cbn in *; auto.
+       (* We try to toggle a door [d]. *)
+       apply one_door_safe_all_doors_safe with (d := d).
+       apply one_door_safe_all_doors_safe with (d' := d) in safe.
+       inversion req0; ssubst.
+       destruct safe as [safe | safe].
     (* 1. The door [d] is closed. Because we are in a trustworthy run, we
           know the door [co d] is also closed, and remains closed. *)
-    ++ right.
-       rewrite tog_equ_2.
-       now apply H2.
+       +++ right.
+           rewrite tog_equ_2.
+           now apply H4.
     (* 2. The door [co d] is closed. Once [d] is toggled, [co d] will remain
           closed. *)
-    ++ right.
-       now rewrite tog_equ_2.
+           +++ right.
+               now rewrite tog_equ_2.
+    ++ cbn in *.
+       eapply H1; [ exact rec | exact safe ].
 Qed.
 
 (** ** Main Theorem *)
 
-Lemma controller_correct
+Lemma controller_correct `{ M1 : MayProvide ix DOORS
+                          , P1 : @Provide ix DOORS M1
+                          , M2 : MayProvide ix (STORE nat)
+                          , P2 : @Provide ix (STORE nat) M2
+                          , @Distinguish ix (STORE nat) DOORS M2 P2 M1
+                          }
   : correct_component controller
                       (no_specs CONTROLLER)
                       doors_specs
-                      (fun _ _ ω => sel left ω = false \/ sel right ω = false).
+                      (fun _ ω => sel left ω = false \/ sel right ω = false).
+
 Proof.
-  intros ωc cpt ωd pred a e req.
+  intros ωc ωd pred a e req.
   split.
   + destruct e.
-    ++ prove_impure; apply close_door_trustworthy.
     ++ prove_impure.
-       apply close_door_trustworthy.
-       apply open_door_trustworthy.
-       now apply close_door_run in Hrun.
-  + intros x st ωj' run.
+       +++ apply close_door_trustworthy.
+       +++ apply close_door_trustworthy.
+    ++ prove_impure.
+       +++ apply close_door_trustworthy.
+       +++ apply open_door_trustworthy.
+           now apply close_door_run in Hrun.
+  + intros x ωj' run.
     split; auto.
-    eapply trustworthy_run_inv; [ exact pred
-                                |  exact run ].
+    eapply trustworthy_run_inv in run; auto.
 Qed.
