core/theories/Core/Notations.v
@@ -1,0 +1,108 @@
+(* FreeSpec
+ * Copyright (C) 2018–2019 ANSSI
+ *
+ * Contributors:
+ * 2018–2019 Thomas Letan <thomas.letan@ssi.gouv.fr>
+ *
+ * This program is free software: you can redistribute it and/or modify
+ * it under the terms of the GNU General Public License as published by
+ * the Free Software Foundation, either version 3 of the License, or
+ * (at your option) any later version.
+ *
+ * This program is distributed in the hope that it will be useful,
+ * but WITHOUT ANY WARRANTY; without even the implied warranty of
+ * MERCHANTABILITY or FITNESS FOR A PARTICULAR PURPOSE.  See the
+ * GNU General Public License for more details.
+ *
+ * You should have received a copy of the GNU General Public License
+ * along with this program. If not, see <http://www.gnu.org/licenses/>.
+ *)
+
+From FreeSpec.Core Require Import Impure.
+
+Generalizable All Variables.
+
+Class Provide2 ix i1 i2 `{Provide ix i1, Provide ix i2}.
+
+#[program]
+Instance Make_Provide2 `(Provide ix i1, Provide ix i2)
+  : Provide2 ix i1 i2.
+
+Class Provide3 ix i1 i2 i3 `{Provide ix i1, Provide ix i2, Provide ix i3}.
+
+#[program]
+Instance Make_Provide3 `(Provide ix i1, Provide ix i2, Provide ix i3)
+  : Provide3 ix i1 i2 i3.
+
+Class Provide4 ix i1 i2 i3 i4
+   `{Provide ix i1, Provide ix i2, Provide ix i3, Provide ix i4}.
+
+#[program]
+Instance Make_Provide4 `{Provide ix i1, Provide ix i2, Provide ix i3, Provide ix i4}
+  : Provide4 ix i1 i2 i3 i4.
+
+Class Provide5 ix i1 i2 i3 i4 i5
+   `{Provide ix i1, Provide ix i2, Provide ix i3, Provide ix i4, Provide ix i5}.
+
+#[program]
+Instance Make_Provide5
+   `{Provide ix i1 , Provide ix i2, Provide ix i3, Provide ix i4, Provide ix i5}
+  : Provide5 ix i1 i2 i3 i4 i5.
+
+Class StrictProvide2 ix i1 i2
+   `{Provide ix i1, Provide ix i2, ! Distinguish ix i1 i2, ! Distinguish ix i2 i1}.
+
+#[program]
+Instance Make_StrictProvide2
+   `(Provide ix i1,  Provide ix i2, ! Distinguish ix i1 i2, ! Distinguish ix i2 i1)
+  : StrictProvide2 ix i1 i2.
+
+Class StrictProvide3 (ix i1 i2 i3 : interface)
+  `{Provide ix i1, Provide ix i2, Provide ix i3, ! Distinguish ix i1 i2,
+    ! Distinguish ix i1 i3, ! Distinguish ix i2 i1, ! Distinguish ix i2 i3,
+    ! Distinguish ix i3 i1, ! Distinguish ix i3 i2}.
+
+#[program]
+Instance Make_StrictProvide3
+  `(Provide ix i1, Provide ix i2, Provide ix i3, ! Distinguish ix i1 i2,
+    ! Distinguish ix i1 i3, ! Distinguish ix i2 i1, ! Distinguish ix i2 i3,
+    ! Distinguish ix i3 i1, ! Distinguish ix i3 i2)
+  : StrictProvide3 ix i1 i2 i3.
+
+Class StrictProvide4 (ix i1 i2 i3 i4 : interface)
+  `{Provide ix i1, Provide ix i2, Provide ix i3, Provide ix i4,
+    ! Distinguish ix i1 i2, ! Distinguish ix i1 i3, ! Distinguish ix i1 i4,
+    ! Distinguish ix i2 i1, ! Distinguish ix i2 i3, ! Distinguish ix i2 i4,
+    ! Distinguish ix i3 i1, ! Distinguish ix i3 i2, ! Distinguish ix i3 i4,
+    ! Distinguish ix i4 i1, ! Distinguish ix i4 i2, ! Distinguish ix i4 i3}.
+
+#[program]
+Instance Make_StrictProvide4
+   `(Provide ix i1, Provide ix i2, Provide ix i3, Provide ix i4,
+    ! Distinguish ix i1 i2, ! Distinguish ix i1 i3, ! Distinguish ix i1 i4,
+    ! Distinguish ix i2 i1, ! Distinguish ix i2 i3, ! Distinguish ix i2 i4,
+    ! Distinguish ix i3 i1, ! Distinguish ix i3 i2, ! Distinguish ix i3 i4,
+    ! Distinguish ix i4 i1, ! Distinguish ix i4 i2, ! Distinguish ix i4 i3)
+  : StrictProvide4 ix i1 i2 i3 i4.
+
+Class StrictProvide5 (ix i1 i2 i3 i4 i5 : interface)
+   `{Provide ix i1, Provide ix i2, Provide ix i3, Provide ix i4, Provide ix i5,
+     ! Distinguish ix i1 i2, ! Distinguish ix i1 i3, ! Distinguish ix i1 i4,
+     ! Distinguish ix i1 i5, ! Distinguish ix i2 i1, ! Distinguish ix i2 i3,
+     ! Distinguish ix i2 i4, ! Distinguish ix i2 i5, ! Distinguish ix i3 i1,
+     ! Distinguish ix i3 i2, ! Distinguish ix i3 i4, ! Distinguish ix i3 i5,
+     ! Distinguish ix i4 i1, ! Distinguish ix i4 i2, ! Distinguish ix i4 i3,
+     ! Distinguish ix i4 i5, ! Distinguish ix i5 i1, ! Distinguish ix i5 i2,
+     ! Distinguish ix i5 i3, ! Distinguish ix i5 i4}.
+
+#[program]
+Instance Make_StrictProvide5 (ix i1 i2 i3 i4 i5 : interface)
+   `(Provide ix i1, Provide ix i2, Provide ix i3, Provide ix i4, Provide ix i5,
+     ! Distinguish ix i1 i2, ! Distinguish ix i1 i3, ! Distinguish ix i1 i4,
+     ! Distinguish ix i1 i5, ! Distinguish ix i2 i1, ! Distinguish ix i2 i3,
+     ! Distinguish ix i2 i4, ! Distinguish ix i2 i5, ! Distinguish ix i3 i1,
+     ! Distinguish ix i3 i2, ! Distinguish ix i3 i4, ! Distinguish ix i3 i5,
+     ! Distinguish ix i4 i1, ! Distinguish ix i4 i2, ! Distinguish ix i4 i3,
+     ! Distinguish ix i4 i5, ! Distinguish ix i5 i1, ! Distinguish ix i5 i2,
+     ! Distinguish ix i5 i3, ! Distinguish ix i5 i4)
+  : StrictProvide5 ix i1 i2 i3 i4 i5.
