stdlib/console/tests/pipe.v
@@ -2,7 +2,7 @@ From FreeSpec Require Import Exec Console.
 
 Generalizable All Variables.
 
-Definition pipe `{ix :| CONSOLE} : impure ix unit :=
+Definition pipe `{Provide ix CONSOLE} : impure ix unit :=
   scan >>= echo.
 
 Exec pipe.
