stdlib/theories/Stdlib/Env.v
@@ -34,10 +34,10 @@ Register ENV as freespec.stdlib.env.type.
 Register GetEnv as freespec.stdlib.env.GetEnv.
 Register SetEnv as freespec.stdlib.env.SetEnv.
 
-Definition get_env `{ix :| ENV} (name : string) : impure ix string :=
+Definition get_env `{Provide ix ENV} (name : string) : impure ix string :=
   request (GetEnv name).
 
-Definition set_env `{ix :| ENV} (name : string) (value : string) : impure ix unit :=
+Definition set_env `{Provide ix ENV} (name : string) (value : string) : impure ix unit :=
     request (SetEnv name value).
 
 Declare ML Module "freespec_stdlib_env".
